imp/example/Stealing.v
@@ -11,89 +11,23 @@ Require Import ModSem Mod ModSemFacts ModFacts.
 Require Import Algebra.
 Require Import SimModSem.
 Require Import ImpPrelude.
+Require Import Mem0.
 Require Import HTactics.
 
 Set Implicit Arguments.
 
 Local Open Scope nat_scope.
 
-(* Module MEM. *)
-
-(*   (* Refer to the memory module in CCR *) *)
-
-(*   Definition callocF : list val -> itree Es val := *)
-(*     fun varg => *)
-(*       sz <- ((pargs [Tint] varg)?);; *)
-(*       m0 <- trigger PGet;; *)
-(*       ` m: Mem.t <- (m0↓)?;; *)
-(*       d <- trigger (Choose _);; *)
-(*       let m1 := Mem.mem_pad m d in *)
-(*       let '(b, m2) := Mem.alloc m1 sz in *)
-(*       trigger (PPut m2↑);;; *)
-(*       Ret (Vptr (inl b) 0). *)
-
-(*   Definition freeF : list val -> itree Es val := *)
-(*     fun varg => *)
-(*       '(b0, ofs) <- ((pargs [Tptr] varg)?);; *)
-(*       ` b: nat <- (unl b0)?;; *)
-(*       m0 <- trigger PGet;; *)
-(*       ` m: Mem.t <- (m0↓)?;; *)
-(*       m1 <- (Mem.free m b ofs)?;; *)
-(*       trigger (PPut m1↑);;; *)
-(*       Ret Vundef. *)
-
-(*   Definition loadF : list val -> itree Es val := *)
-(*     fun varg => *)
-(*       '(b, ofs) <- ((pargs [Tptr] varg)?);; *)
-(*       m0 <- trigger PGet;; *)
-(*       ` m: Mem.t <- (m0↓)?;; *)
-(*       v <- (Mem.load m b ofs)?;; *)
-(*       Ret v. *)
-
-(*   Definition storeF : list val -> itree Es val := *)
-(*     fun varg => *)
-(*       '(b, ofs, v) <- ((pargs [Tptr; Tuntyped] varg)?);; *)
-(*       m0 <- trigger PGet;; *)
-(*       ` m: Mem.t <- (m0↓)?;; *)
-(*       m1 <- (Mem.store m b ofs v)?;; *)
-(*       trigger (PPut m1↑);;; *)
-(*       Ret Vundef. *)
-
-(*   Definition cmpF : list val -> itree Es val := *)
-(*     fun varg => *)
-(*       '(v0, v1) <- ((pargs [Tuntyped; Tuntyped] varg)?);; *)
-(*       m0 <- trigger PGet;; *)
-(*       ` m: Mem.t <- (m0↓)?;; *)
-(*       b <- (vcmp m v0 v1)?;; *)
-(*       if (b: bool) then Ret (Vint 1%Z) else Ret (Vint 0%Z). *)
-
-(*   Definition memMS_ (sk: Sk.t) : ModSem._t := *)
-(*     {| *)
-(*       ModSem.fnsems := *)
-(*       [("calloc", cfunU callocF); ("free", cfunU freeF); *)
-(*        ("load", cfunU loadF); ("store", cfunU storeF); ("cmp", cfunU cmpF)]; *)
-(*       ModSem.initial_st := (Mem.load_mem sk)↑; *)
-(*     |}. *)
-
-(*   Definition memMS (sk: Sk.t) : ModSem.t := Algebra.just (memMS_ sk). *)
-
-(*   Definition memM: Mod.t := *)
-(*     {| *)
-(*       Mod.get_modsem := memMS; *)
-(*       Mod.sk := Sk.unit; *)
-(*     |}. *)
-
-(* End MEM. *)
 
 Module VAR0.
 
-  (* TODO: store 0 *)
   Definition initF : list val -> itree Es val :=
     fun varg =>
       _ <- ((pargs [] varg)?);;
       ` ptr: val <- ccallU "alloc" [Vint 1%Z];;
+      ` _ : val <- ccallU "store" [ptr; (Vint 0%Z)];;
       _ <- trigger (PPut ptr↑);;
-      Ret Vundef.
+      Ret (Vint 0).
 
   Definition getF : list val -> itree Es val :=
     fun varg =>
@@ -118,3 +52,164 @@ Module VAR0.
   Definition varMS : ModSem.t := Algebra.just varMS_.
 
 End VAR0.
+
+Module VAR1.
+
+  Definition initF : list val -> itree Es val :=
+    fun varg =>
+      _ <- ((pargs [] varg)?);;
+      _ <- trigger (PPut (Some (Vint 0%Z))↑);;
+      Ret (Vint 0).
+
+  Definition getF : list val -> itree Es val :=
+    fun varg =>
+      _ <- ((pargs [] varg)?);;
+      v0 <- trigger (PGet);;
+      ` v1: (option val) <- (v0↓)?;;
+      ` v: val <- v1?;;
+      Ret v.
+
+  Definition setF : list val -> itree Es val :=
+    fun varg =>
+      w <- ((pargs [Tint] varg)?);;
+      v0 <- trigger (PGet);;
+      ` _: (option val) <- (v0↓)?;;
+      _ <- trigger (PPut (Some (Vint w))↑);;
+      Ret (Vint 0).
+
+  Definition varMS_ : ModSem._t :=
+    {|
+      ModSem.fnsems := [("init", cfunU initF); ("get", cfunU getF); ("set", cfunU setF)];
+      ModSem.initial_st := (@None val)↑;
+    |}.
+
+  Definition varMS : ModSem.t := Algebra.just varMS_.
+
+End VAR1.
+
+Section PROOFSIM.
+
+  Import ModSemPair.
+
+  Ltac ired_eq_l := (Red.prw IRed._red_gen 2 0).
+  Ltac ired_eq_r := (Red.prw IRed._red_gen 1 0).
+
+  Definition mem_less_defined (m0 m1: Mem.t) :=
+    forall b ofs, (Mem.cnts m0 b ofs = None) -> (Mem.cnts m1 b ofs = None).
+
+  Definition var_sim_inv : nat -> (Any.t * Any.t) -> Prop :=
+    fun n '(s, t) =>
+      match n with
+      | O =>
+          exists (m: Mem.t),
+          (<<SRC: s = Any.pair (m↑) ((@None val)↑)>>) /\
+            (<<TGT: t = Any.pair (m↑) (Vnullptr↑)>>) /\
+            (<<WFM: Mem.wf m>>)
+      | S _ =>
+          exists (v: val) (ms mt: Mem.t) (b: nat) (ofs: Z),
+          (<<SRC: s = Any.pair (ms↑) ((Some v)↑)>>) /\
+            (<<TGT: t = Any.pair (mt↑) ((Vptr (inl b) ofs)↑)>>) /\
+            (<<VART: Mem.load mt (inl b) ofs = Some v>>) /\
+            (<<VARS: forall ofs0, Mem.cnts ms (inl b) ofs0 = None>>) /\
+            (<<WFMS: Mem.wf ms>>) /\
+            (<<WFMT: Mem.wf mt>>) /\
+            (<<NBLK: exists nbd, (Mem.nb mt) = (Mem.nb ms) + nbd>>) /\
+            (<<MLD: mem_less_defined mt ms>>)
+      end.
+
+  Ltac unfold_goal H :=
+    match goal with
+    | [|- gpaco8 (_sim_itree ?_temp1 _ _) (cpn8 (_sim_itree ?_temp2 _ _)) _ _ _ _ _ _ _ _ _ _] =>
+        let tvar1 := fresh "temp1" in
+        let tvar2 := fresh "temp2" in
+        remember _temp1 as tvar1; remember _temp2 as tvar2; unfold H; subst tvar1 tvar2
+    end.
+
+  Ltac hide_src :=
+    match goal with
+    | [ |- (gpaco8 (_sim_itree _ _ _) _ _ _ _ _ _ _ _ _ (_, ?i_src) (_, _)) ] =>
+        let hsrc := fresh "hide_src" in set i_src as hsrc at 1
+    end.
+
+  Ltac hide_tgt :=
+    match goal with
+    | [ |- (gpaco8 (_sim_itree _ _ _) _ _ _ _ _ _ _ _ _ (_, _) (_, ?i_tgt)) ] =>
+        let htgt := fresh "hide_tgt" in set i_tgt as htgt at 2
+    end.
+
+  Lemma var_sim:
+    ModSemPair.sim ((MemSem Sk.unit) ⊕ VAR1.varMS) ((MemSem Sk.unit) ⊕ VAR0.varMS).
+  Proof.
+    Local Opaque String.eqb.
+    ss. eapply (@mk _ _ _ var_sim_inv _ Nat.le_preorder).
+    { i. ss. des; clarify.
+      - exists (focus_left (T:=Any.t) ∘ cfunU allocF). split. auto. ii. subst y.
+        ginit.
+        unfold_goal @allocF. unfold_goal @cfunU.
+        destruct w; ss.
+        { des. hide_tgt. steps. subst hide_tgt. steps.
+          (* TODO *)
+
+        
+        
+        unfold RPT1.rptF. unfold RPT0.rptF at 2. unfold cfunU at 3 4.
+        unfold sim_fsem. ii. subst y.
+        ginit.
+        unfold cfunU at 5. steps.
+        destruct p0. unfold unptr, unint, unr in *. des_ifs_safe. ss; clarify.
+        destruct (eqb_spec "succ" s).
+        2:{ steps. }
+        clarify.
+        steps. force_r. eexists; auto.
+        steps. rename z0 into v.
+        remember (Z.to_nat z) as n.
+        revert x z v _UNWRAPU _ASSUME Heqn. induction n; intros.
+        { hexploit Z_to_nat_le_zero; eauto. intros. des_ifs.
+          2:{ lia. }
+          ss. steps.  unfold lift_rel. exists w; auto.
+        }
+        { hexploit Z_to_nat_ge_one; eauto. intros ZRANGE. des_ifs. clear l.
+          ss.
+          unfold ccallU. steps.
+          { right; left. instantiate (1:=focus_right (T:=Any.t) ∘ cfunU SUCC.succF). f_equal. }
+          unfold cfunU at 5. steps.
+          rewrite ! SUCC.red_succF. steps.
+          { left. instantiate (1:= focus_left (T:=Any.t) ∘ cfunU RPT0.rptF). auto. }
+          unfold cfunU at 5. steps. unfold RPT0.rptF at 3. steps.
+          force_r.
+          { clear - _ASSUME ZRANGE. unfold_intrange_64.
+            des_ifs. apply sumbool_to_bool_true in _ASSUME, H.
+            apply andb_true_intro. split; apply sumbool_to_bool_is_true; lia.
+          }
+          steps.
+          specialize (IHn ([Vptr (inr "succ") 0; Vint (z - 1); Vint (v +1)]↑) (z - 1)%Z (v + 1)%Z).
+          hexploit IHn; auto.
+          { apply Any.upcast_downcast. }
+          { lia. }
+          clear IHn; intros IHn. des_ifs.
+          { steps.
+            match goal with
+            | [IHn: gpaco8 _ _ _ _ _ _ _ _ _ _ _ (?t1) |-
+                 gpaco8 _ _ _ _ _ _ _ _ _ _ _ (?t2)] =>
+                replace t2 with t1
+            end.
+            guclo lflagC_spec. econs. eapply IHn.
+            all: auto.
+            f_equal. ired_eq_l. auto.
+          }
+          { steps. irw in IHn.
+            guclo guttC_spec. econs.
+            { guclo lflagC_spec. econs. eapply IHn. all: auto. }
+            - apply Reflexive_eqit_eq.
+            - ired_eq_r.
+              apply eqit_bind. apply Reflexive_eqit_eq. ii.
+              apply eqit_bind. apply Reflexive_eqit_eq. ii.
+              ired_eq_l. apply eqit_Tau_l. ired_eq_l. ired_eq_r.
+              apply Reflexive_eqit_eq.
+          }
+        }
+    }
+    { ss. exists O. auto. }
+  Qed.
+
+End PROOFSIM.
